\documentclass[../MAS242_Note.tex]{subfiles}

\begin{document}
\section{Calculus of Series Functions}

\thm[limDiff]{}{
    Given a sequence \(\{f_j\}_{j \in \NN} \subseteq \RR[(a,b)]\)
    of differentiable functions, suppose the following.
    \begin{enumerate}[nolistsep, label=(\roman*)]
        \ii \(\{f_j(x_0)\}_{j \in \NN} \subseteq \RR\) converges for some \(x_0 \in (a, b)\).
        \ii \(\{f_j'\}_{j \in \NN} \subseteq \RR[(a,b)]\) uniformly converges on \((a, b)\).
    \end{enumerate}
    Then, \(f_j \rightrightarrows f\) for some \(f \colon (a, b) \to \RR\) on \((a, b)\).
    Furthermore, \(f\) is differentiable on \((a, b)\) and
    \(\fall x \in (a, b),\: f'(x) = \lim_{j \to \infty} f_j'(x)\).
}
\pf{Proof}{
    We shall first show the uniform convergence of \(\{f_j\}\).
    Take any \(\veps \in \RR_+\).
    Then, there exists \(N \in \NN\) such that, for all \(j, k \ge N\),
    \[
        \big(|f_j(x_0)-f_k(x_0)| < \veps/2\big)
        \land \big(\fall x \in (a, b),\:|f_j'(x) - f_k'(x)| < \veps/2(b-a)\big).
    \]
    By MVT, for all \(x, \tilde{x} \in (a, b)\) with \(x \neq \tilde x\),
    there exists \(x_\ast \in (a, b)\) such that
    \[
        (f_j-f_k)(x)-(f_j-f_k)(\tilde x) = (f_j-f_k)'(x_\ast) \cdot (x-\tilde x)
    \]
    Hence, \(|(f_j-f_k)(x)-(f_j-f_k)(\tilde x)| < \veps/2\).
    Therefore, \(|(f_j-f_k)(x)| < \veps\) by triangle inequality obtained by setting \(\tilde x = x_0\).
    This directly implies that \(\{f_j\}\) is uniformly Cauchy and thus uniformly converges
    by \Cref{lem:unifConvIff}. \checkmark

    Let \(f_j \to f\). Fixing \(x \in (a, b)\), define
    \[
        \psi_j(t) \triangleq \frac{f_j(t) - f_j(x)}{t-x} \quad\text{and}\quad
        \psi(t) \triangleq \frac{f(t) - f(x)}{t-x}
    \]
    for \(t \in (a, b)\) and \(t \neq x\). Now, we claim that \(\{\psi_j\}_{j \in \NN}\)
    is uniformly Cauchy. Take any \(\veps \in \RR_+\).
    Then, for \(j, k \ge N\),
    \[
        |\psi_j(t) - \psi_k(t)| = \left|\frac{(f_j-f_k)(t)-(f_j-f_k)(x)}{t-x}\right|
        < \frac{\veps}{2(b-a)}.
    \]
    Hence, \(\{\psi_j\}\) uniformly converges by \Cref{lem:unifConvIff},
    and \(\psi_j \to \psi\) as \(f_j \to f\).

    Let \(A_j \triangleq \lim_{t \to x} \psi_j(t) = f_j'(x)\).
    By the supposition (ii), we have convergence of \(\{A_j\}_{j \in \NN}\).
    Now, we claim that \(\lim_{t \to x} \psi(t) = \lim_{j \to \infty} A_j\).
    Let \(A_j \to A\). Take any \(\veps \in \RR_+\).
    There exists \(N' \in \NN\) such that, if \(j \ge N'\),
    we have \(|\psi(t) - \psi_j(t)| < \veps/3\) for all \(t \in (a, b) \setminus \{x\}\)
    ana \(|A_j - A| < \veps/3\).
    In addition, from the definition of \(A_j\), there exists \(\delta \in \RR_+\)
    such that, whenever \(0 < |t - x| < \delta\), we have \(|\psi_{N'}(t)-A_{N'}| < \veps/3\).
    Now, we have
    \[
        |\psi(t) - A| \le |\psi(t) - \psi_{N'}(t)| + |\psi_{N'}(t) - A_{N'}| + |A_{N'}-A| < \veps
    \]
    for \(0 < |t-x| < \delta\).
    Hence, \(f'(x) = \lim_{t \to x} \psi(t) = \lim_{j \to \infty} f_j'(x)\).
}

\cor[tbtDiff]{Term-by-Term Differentiation}{
    Given a sequence \(\{f_j\}_{j \in \NN} \subseteq \RR[(a,b)]\)
    of differentiable functions, let \(F_n = \sum_{j=1}^{n} f_j\).
    Suppose the following.
    \begin{enumerate}[nolistsep, label=(\roman*)]
        \ii \(\{F_n(x_0)\}_{n \in \NN} \subseteq \RR\) converges for some \(x_0 \in (a, b)\).
        \ii \(\{F_n'\}_{n \in \NN} \subseteq \RR[(a,b)]\) uniformly converges on \((a, b)\).
    \end{enumerate}
    Then, \(\{F_n\}\) converges uniformly to a function \(F \colon (a, b) \to \RR\)
    on \((a, b)\).
    Furthermore, \(F\) is differentiable on \((a, b)\) and
    \(\fall x \in (a, b),\: F'(x) = \sum_{j=1}^{\infty} f_j'(x)\).
}

\exmp{}{
    Let \(f_j(x) = \sin(x/j^2)\) for \(-1 < x < 1\)
    and \(F_n = \sum_{j=1}^{n} f_j\).

    For \(x_0 = 0\),  the sequence \(\{F_n(x_0)\}_{n \in \NN}\) converges (to zero).
    Now, we have \(F_n'(x) = \sum_{j=1}^{n} \cos(x/j^2)/j^2\).
    Then,   for \(n, m \in \NN\) with \(m \ge n\),
    \(|F_m'(x) - F_n'(x)| \le \sum_{j=n+1}^{m} 1/j^2 \to 0\) as \(n, m \to \infty\).
    Hence, \(\{F_n'\}\) is uniformly Cauchy; and thus it converges uniformly by \Cref{lem:unifConvIff}.
    Hence, \Cref{cor:tbtDiff} guarantees the uniform convergence and differentiability of
    \(\sum_{j=1}^{\infty} f_j\).
}

\thm[]{}{
    Given a sequence \(\{f_j\}_{j \in \NN} \subseteq \RR[(a,b)]\)
    of functions Riemann integrable on \((a, b)\),
    if \(f_j \rightrightarrows f\) on \((a, b)\), then \(f\) is Riemann integrable on \((a, b)\).
    Furthermore, \(\int_{a}^{b} f(x) \d x = \lim_{j \to \infty} \int_{a}^{b} f_j(x) \d x\).
}
\pf{Proof}{
    
}

\cor[tbtInt]{Term-by-Term Integration}{
    Given a sequence \(\{f_j\}_{j \in \NN} \subseteq \RR[(a,b)]\)
    of functions Riemann integrable on \((a, b)\),
    suppose \(\sum f_j \rightrightarrows F\) for some \(F \colon (a, b) \to \RR\).
    Then, \(\int_{a}^{b} F(x)\d x = \lim_{n \to \infty} \int_{a}^{b} \sum_{j=1}^{n} f_j(x) \d x\).
}

\thm[]{}{
    Given a power series \(\sum_{j=0}^{\infty} c_j x^j\),
    let
    \[
        \alpha \triangleq \limsup_{n \to \infty} \sqrt[n]{|c_n|}, \quad
        R \triangleq \frac{1}{\alpha}.
    \]
    (If \(\alpha = 0\), put \(R = \infty\); if \(\alpha = \infty\), put \(R = 0\).)
    Then, \(\sum c_j x^j\) converges if \(|x| < R\), and diverges if \(|x| > R\).
}
\pf{Proof}{
    We have
    \[
        \limsup_{n \to \infty} \sqrt[n]{|c_n x^n|}
        = \alpha |x|,
    \]
    therefore the result follows from the root test.
}

\thm[]{}{
    Given a power series \(P(x) = \sum_{j=0}^{\infty} c_j x^j\),
    let \(R\) be the radius of convergence.
    Then, for any \(\veps \in (0, R)\),
    \(P(x)\) uniformly
    converges on \([-R+\veps, R-\veps]\).
}

\nt{
    TODO: write proofs for
    \begin{itemize}[nolistsep]
        \ii Radius of convergence of \(P'(x)\) equals the radius of convergence of \(P(x)\).
        \ii For all \(|x-x_0| < R\), we have \(P^{(k)}(x) = \sum_{j=k}^{\infty} j(j-1)\cdots(j-k+1)(x-x_0)^{j-k}\).
    \end{itemize}
}

\thm[taylorThm]{Taylor's Theorem}{
    Suppose a function \(f(x)\) is represented as a power series \(f(x) = \sum_{j=0}^{\infty} c_jx^j\)
    and that the radius of convergence is \(R \in [0, \infty]\).
    Then, for any \(x \in (-R, R)\),
    \[
        |x - a| < R - |a| \implies f(x) = \sum_{j=0}^{\infty} \frac{f^{(j)}(a)}{j!} (x-a)^j.
    \]
}
\pf{Proof}{
    Fix \(a \in (-R, R)\).
    Suppose that \(f(x) = \sum_{j=0}^{\infty} \mu_j (x-a)^j\).
    By corollary, \(f^{(k)}(x) = \sum_{j=k}^{\infty} j(j-1)\cdots(j-k+1) \mu_j(x-x_0)^{j-k}\).

    \[\begin{aligned}[t]
        f(x) &= \sum_{j=0}^{\infty} c_j \big((x-a)+a\big)^{j} \\
             &= \sum_{j=0}^{\infty} \sum_{k=0}^{j} c_j \binom{j}{k} a^{j-k}(x-a)^k
             = \sum_{k=0}^{\infty} \left[\sum_{j=k}^{\infty} c_j \binom{j}{k} a^{j-k}\right](x-a)^k.
    \end{aligned}\]
    The rearrangement is valid when \(T(x) = \sum_{j=0}^{\infty} \sum_{k=0}^{j} \big| c_j \binom{j}{k} a^{j-k}(x-a)^k \big|
    = \sum_{j=0}^{\infty} |c_j| (|x-a|+|a|)^j\) converges, i.e.,
    when \(\limsup_{j \to \infty} \big\{ |c_j| (|x-a|+|a|)^j \big\}^{1/j} = (|x-a|+|a|) / R < 1\).
    Hence, \(f(x) = \sum_{j=0}^{\infty} \mu_j (x-a)^j\) converges when \(|x-a| < R - |a|\).
}

\nt{
    \noindent
    \Cref{th:taylorThm} implies that every series function is \(C^\infty\) and analytic.
}

\nt{
    We do not have a reliable method to determine the convergence at the boundary points,
    we have at least a theorem for the situation in which the convergence is given.
}

\thm{}{
    Let \(P(x) = \sum_{j=0}^{\infty} c_j(x-x_0)^j\) be a power series and let
    \(0 < R < \infty\) be its radius of convergence.
    If \(P(x)\) converges at \(x = x_0 + R\),
    then, \(P(x)\) uniformly converges on \([x_0, x_0 + R]\).
}
\pf{Proof}{
    For convenience, rescale \(P(x)\) by setting
    \(Q \big(\frac{x-x_0}{R}\big) = P(x)\),
    so \(Q(z) = \sum_{j=0}^{\infty} R^{j}c_j z^j\),
    and the radius of convergence of \(Q\) is \(1\)
    and \(Q(z)\) converges at \(z = 1\).
    Hence, we are left to prove the uniform convergence of \(Q(z)\) on \([0, 1]\).

    Let \(\tilde{c}_j = R^jc_j\) so \(Q(z) = \sum_{j=0}^{\infty} \tilde{c}_j z^j\).
    Let \(Q_n(z) = \sum_{j=0}^{n} \tilde c_j z^j\) and \(S_n = Q_n(1) = \sum_{j=0}^{n} \tilde c_j\).
    Take any \(\veps \in \RR_+\). Then, there exists \(N \in \NN\) such that
    \(|S_j - S_k| < \veps/3\) for all \(j, k \ge N\).
    For \(n, m \in \NN\) with \(m > n\),
    \[\begin{aligned}[t]
        Q_m(z) - Q_n(z) &= \textstyle \big( S_m z^{m+1} - \sum_{j=0}^{m} S_j (z^{j+1} - z^j) \big)
                            - \big( S_n z^{n+1} - \sum_{j=0}^{n} S_j (z^{j+1} - z^j) \big) \\
                        &= \textstyle \sum_{j=n+1}^{m} S_j(z^j - z^{j+1}) + (S_m z^{m+1} - S_n z^{n+1}) \\
                        &= \textstyle \sum_{j=n+1}^{m} S_j(z^j - z^{j+1})
                            - S_n \sum_{j=n+1}^{m} (z^{j} - z^{j+1})
                            + (S_m - S_n) z^{m+1}\\
                        &= \textstyle \sum_{j=n+1}^{m} (S_j - S_n)(z^j - z^{j+1}) + (S_m - S_n) z^{m+1}.
    \end{aligned}\]
    Hence, for all \(m > n \ge N\) and \(z \in [0, 1]\),
    \[
        |Q_m(z) - Q_n(z)| \le \textstyle \sum_{j=n+1}^{m} (\veps/3) (z^j - z^{j+1}) + \veps/3
                          = (\veps/3) (z^{n+1} - z^{m+1}) + \veps/3 < \veps.
    \]
    Hence, \(Q(z)\) uniformly converges on \([0, 1]\) by \Cref{lem:unifConvIff}.
}

\end{document}
