\documentclass[../introduction_to_set_theory.tex]{subfiles}

\begin{document}

\subsection*{Selected Problems}

\exer[3.1.1]{}{
    \begin{enumerate}[nolistsep, label=(\roman*), leftmargin=*]
        \ii \(\fall x,\: x \subseteq S(x)\)
        \ii \(\fall x,\: \lnot(\exs z,\: x \subsetneq z \subsetneq S(x))\)
    \end{enumerate}
}
\mclm{Proof}{\hfill
\begin{enumerate}[nolistsep, label=(\roman*)]
    \ii
    \(x \subseteq x \subseteq x \cup \{x\} = S(x)\)

    \ii
    Take any \(z\) such that such that \(x \subseteq z \subseteq S(x) = x \cup \{x\}\).
    If \(z \subseteq x\), then we have \(z = x\).
    If \(z \not\subseteq x\), then there exists \(y\) such that
    \(y \in z\) and \(y \notin x\).
    However, \(y \in x \cup \{x\}\), and thus \(y = x\).
    Therefore, \(S(x) \subseteq z\); \(z = S(x)\).
    In conclusion, any \(z\) such that \(x \subseteq z \subseteq S(x)\)
    must satisfy \(z = x\) or \(z = S(x)\).
    \qed
\end{enumerate}
}

\end{document}
